\documentclass[12pt]{article}
\usepackage{amsmath}
\usepackage{amssymb} %mathbb
\usepackage{graphicx}
\usepackage{hyperref}
\usepackage[latin1]{inputenc}
\usepackage[top=1.0cm,bottom=1.3cm,left=1.0cm,right=1.0cm]{geometry}

\begin{document}

\begin{align}
  x &= \cfrac{1}{a + \sqrt{b} + \sqrt{c} + \sqrt{d}} \cdot \cfrac{a + \sqrt{b} - \sqrt{c} - \sqrt{d}}{a + \sqrt{b} - \sqrt{c} - \sqrt{d}} \\
    &= \cfrac{a + \sqrt{b} - \sqrt{c} - \sqrt{d}}{(a + \sqrt{b})^2 - (\sqrt{c} + \sqrt{d})^2} \\
    &= \cfrac{a + \sqrt{b} - \sqrt{c} - \sqrt{d}}{a^2 + 2a\sqrt{b} + b - c - 2\sqrt{cd} - d} \cdot \cfrac{a^2 + b - c - d + 2a\sqrt{b} + 2\sqrt{cd}}{a^2 + b - c - d + 2a\sqrt{b} + 2\sqrt{cd}} \\
    &= \cfrac{P_1(b, c, d, cd)}{(a^2 + b - c - d + 2a\sqrt{b})^2 - 4cd} \\
    &= \cfrac{P_1}{(a^2 + b - c - d)^2 + 4a(a^2 + b - c - d)\sqrt{b} + 4a^2 b - 4cd} \\
    &= \cfrac{P_1}{F + G\sqrt{b}} \cdot \cfrac{F - G\sqrt{b}}{F - G\sqrt{b}} \\
    &= \cfrac{P_2}{F^2 - bG^2} = x \\
  F &= (a^2 + b - c - d)^2 + 4a^2 b - 4cd \\
  G &= 4a(a^2 + b - c - d) \\
  P_1 &= (a + \sqrt{b} - \sqrt{c} - \sqrt{d})(a^2 + b - c - d + 2a\sqrt{b} + 2\sqrt{cd}) \\
  P_2 &= P_1 (F - G\sqrt{b})
\end{align}

\vspace{6mm}

Out of charity, there is no salvation at all.

Vinicius Claudino Ferraz. 2020/July/24

\end{document}